# Self-Correcting LLM Coding Workflow Results

## Initial Query
```
Reverse a string without using the built-in reverse function
```

## Attempts
### Attempt 1/2
#### Generated Function
```python
def reverse_string(s):
    # Initialize an empty string for the reversed version
    reversed_s = ""
    
    # Iterate over the original string in reverse order
    for char in range(len(s) - 1, -1, -1):
        reversed_s += s[char]
        
    return reversed_s

# Example usage
original_string = "Hello, World!"
reversed_string = reverse_string(original_string)
print("Original String:", original_string)
print("Reversed String:", reversed_string)

# Test case
def test_reverse_string():
    test_string = "python"
    assert reverse_string(test_string) == "nohtyp", f"Test failed! Expected 'nohtyp' but got {reverse_string(test_string)}"
    print("Test passed!")

test_reverse_string()  # Running the test case
```

#### Test Case
```python

```

#### Example Usage
```python
def reverse_string(s):
    # Initialize an empty string for the reversed version
    reversed_s = ""
    
    # Iterate over the original string in reverse order
    for char in range(len(s) - 1, -1, -1):
        reversed_s += s[char]
        
    return reversed_s

# Example usage
original_string = "Hello, World!"
reversed_string = reverse_string(original_string)
print("Original String:", original_string)
print("Reversed String:", reversed_string)

# Test case
def test_reverse_string():
    test_string = "python"
    assert reverse_string(test_string) == "nohtyp", f"Test failed! Expected 'nohtyp' but got {reverse_string(test_string)}"
    print("Test passed!")

test_reverse_string()  # Running the test case
```

## Final Results
### Success: Function passed all tests
#### Final Function
```python
def reverse_string(s):
    # Initialize an empty string for the reversed version
    reversed_s = ""
    
    # Iterate over the original string in reverse order
    for char in range(len(s) - 1, -1, -1):
        reversed_s += s[char]
        
    return reversed_s

# Example usage
original_string = "Hello, World!"
reversed_string = reverse_string(original_string)
print("Original String:", original_string)
print("Reversed String:", reversed_string)

# Test case
def test_reverse_string():
    test_string = "python"
    assert reverse_string(test_string) == "nohtyp", f"Test failed! Expected 'nohtyp' but got {reverse_string(test_string)}"
    print("Test passed!")

test_reverse_string()  # Running the test case
```

#### Example Usage
```python
def reverse_string(s):
    # Initialize an empty string for the reversed version
    reversed_s = ""
    
    # Iterate over the original string in reverse order
    for char in range(len(s) - 1, -1, -1):
        reversed_s += s[char]
        
    return reversed_s

# Example usage
original_string = "Hello, World!"
reversed_string = reverse_string(original_string)
print("Original String:", original_string)
print("Reversed String:", reversed_string)

# Test case
def test_reverse_string():
    test_string = "python"
    assert reverse_string(test_string) == "nohtyp", f"Test failed! Expected 'nohtyp' but got {reverse_string(test_string)}"
    print("Test passed!")

test_reverse_string()  # Running the test case
```
